<?xml version="1.0"?>
<rdf:RDF xmlns="https://github.com/razpotnik/bubo#"
     xml:base="https://github.com/razpotnik/bubo"
     xmlns:owl="http://www.w3.org/2002/07/owl#"
     xmlns:rdf="http://www.w3.org/1999/02/22-rdf-syntax-ns#"
     xmlns:xml="http://www.w3.org/XML/1998/namespace"
     xmlns:xsd="http://www.w3.org/2001/XMLSchema#"
     xmlns:bubo="https://github.com/razpotnik/bubo#"
     xmlns:rdfs="http://www.w3.org/2000/01/rdf-schema#">
    <owl:Ontology rdf:about="https://github.com/razpotnik/bubo">
        <rdfs:comment>BuBO - Build graph Based Ontology: An OWL ontology of AOSP build system dependencies.</rdfs:comment>
    </owl:Ontology>
    


    <!-- 
    ///////////////////////////////////////////////////////////////////////////////////////
    //
    // Object Properties
    //
    ///////////////////////////////////////////////////////////////////////////////////////
     -->

    


    <!-- https://github.com/razpotnik/bubo#BuildsModule -->

    <owl:ObjectProperty rdf:about="https://github.com/razpotnik/bubo#BuildsModule">
        <rdfs:subPropertyOf rdf:resource="http://www.w3.org/2002/07/owl#topObjectProperty"/>
        <rdfs:domain rdf:resource="https://github.com/razpotnik/bubo#BuildFile"/>
        <rdfs:range rdf:resource="https://github.com/razpotnik/bubo#Module"/>
        <rdfs:comment>BuildsModule represents a build file building a module.</rdfs:comment>
    </owl:ObjectProperty>
    


    <!-- https://github.com/razpotnik/bubo#DependsOn -->

    <owl:ObjectProperty rdf:about="https://github.com/razpotnik/bubo#DependsOn">
        <rdfs:subPropertyOf rdf:resource="http://www.w3.org/2002/07/owl#topObjectProperty"/>
        <rdf:type rdf:resource="http://www.w3.org/2002/07/owl#TransitiveProperty"/>
        <rdfs:comment>DependsOn is the main relationship of BuBO, representing a dependency between two classes (a module or build file, which can depend on build files or libraries).</rdfs:comment>
    </owl:ObjectProperty>
    


    <!-- 
    ///////////////////////////////////////////////////////////////////////////////////////
    //
    // Data properties
    //
    ///////////////////////////////////////////////////////////////////////////////////////
     -->

    


    <!-- https://github.com/razpotnik/bubo#filePath -->

    <owl:DatatypeProperty rdf:about="https://github.com/razpotnik/bubo#filePath">
        <rdfs:subPropertyOf rdf:resource="http://www.w3.org/2002/07/owl#topDataProperty"/>
        <rdfs:domain rdf:resource="https://github.com/razpotnik/bubo#BuildFile"/>
        <rdfs:range rdf:resource="http://www.w3.org/2001/XMLSchema#string"/>
    </owl:DatatypeProperty>
    


    <!-- 
    ///////////////////////////////////////////////////////////////////////////////////////
    //
    // Classes
    //
    ///////////////////////////////////////////////////////////////////////////////////////
     -->

    


    <!-- https://github.com/razpotnik/bubo#AndroidLibrary -->

    <owl:Class rdf:about="https://github.com/razpotnik/bubo#AndroidLibrary">
        <rdfs:subClassOf rdf:resource="https://github.com/razpotnik/bubo#Library"/>
        <owl:disjointWith rdf:resource="https://github.com/razpotnik/bubo#JavaLibrary"/>
        <rdfs:comment>AndroidLibrary represents an Android library.</rdfs:comment>
    </owl:Class>
    


    <!-- https://github.com/razpotnik/bubo#BlueprintFile -->

    <owl:Class rdf:about="https://github.com/razpotnik/bubo#BlueprintFile">
        <rdfs:subClassOf rdf:resource="https://github.com/razpotnik/bubo#BuildFile"/>
        <owl:disjointWith rdf:resource="https://github.com/razpotnik/bubo#Makefile"/>
        <rdfs:comment>BlueprintFile represents a Blueprint file, commonly Android.bp, used by Soong to define modules.</rdfs:comment>
    </owl:Class>
    


    <!-- https://github.com/razpotnik/bubo#BuildFile -->

    <owl:Class rdf:about="https://github.com/razpotnik/bubo#BuildFile">
        <rdfs:comment>BuildFile represents a build configuration script, e.g. Makefile, Blueprint file, in AOSP.</rdfs:comment>
    </owl:Class>
    


    <!-- https://github.com/razpotnik/bubo#JavaLibrary -->

    <owl:Class rdf:about="https://github.com/razpotnik/bubo#JavaLibrary">
        <rdfs:subClassOf rdf:resource="https://github.com/razpotnik/bubo#Library"/>
        <rdfs:comment>JavaLibrary represents a Java library.</rdfs:comment>
    </owl:Class>
    


    <!-- https://github.com/razpotnik/bubo#Library -->

    <owl:Class rdf:about="https://github.com/razpotnik/bubo#Library">
        <rdfs:comment>Library represents a library. It has two types, Android libraries and Java libraries.</rdfs:comment>
    </owl:Class>
    


    <!-- https://github.com/razpotnik/bubo#Makefile -->

    <owl:Class rdf:about="https://github.com/razpotnik/bubo#Makefile">
        <rdfs:subClassOf rdf:resource="https://github.com/razpotnik/bubo#BuildFile"/>
        <rdfs:comment>Makefile represents a Makefile, used in AOSP by Make/Kati to define build rules and handle dependencies.</rdfs:comment>
    </owl:Class>
    


    <!-- https://github.com/razpotnik/bubo#Module -->

    <owl:Class rdf:about="https://github.com/razpotnik/bubo#Module">
        <rdfs:comment>Module represents an Android module</rdfs:comment>
    </owl:Class>
    


    <!-- 
    ///////////////////////////////////////////////////////////////////////////////////////
    //
    // General axioms
    //
    ///////////////////////////////////////////////////////////////////////////////////////
     -->

    <rdf:Description>
        <rdf:type rdf:resource="http://www.w3.org/2002/07/owl#AllDisjointClasses"/>
        <owl:members rdf:parseType="Collection">
            <rdf:Description rdf:about="https://github.com/razpotnik/bubo#BuildFile"/>
            <rdf:Description rdf:about="https://github.com/razpotnik/bubo#Library"/>
            <rdf:Description rdf:about="https://github.com/razpotnik/bubo#Module"/>
        </owl:members>
    </rdf:Description>
</rdf:RDF>



<!-- Generated by the OWL API (version 4.5.29.2024-05-13T12:11:03Z) https://github.com/owlcs/owlapi -->

